\documentclass[10pt]{article}

\input{../templates/set.tex}

\title{MATH 240: Discrete Structures - Assignment 3}
\author{Liam Scalzulli\\
\href{mailto:liam.scalzulli@mail.mcgill.ca}{liam.scalzulli@mail.mcgill.ca}}
\date{\today}

\begin{document}
\maketitle

\subsection*{Problem 1}

\begin{proof}
  Assume $2^n - 1$ is prime. \spacing

  \noindent
  Let $\sigma(n)$ be a function that computes the sum of all divisors of a given
  number $n$.
  \spacing

  \noindent
  Then $\sigma(2^n - 1) = 2^n$ since the only divisors of $2^n - 1$ are $1$ and $2 ^ n - 1$ as a result
  of $2^n - 1$ being prime:

  $$ 1 + 2^{n} - 1 = 2^{n} $$

  \noindent
  Moreover, we have $\sigma(2^{n - 1}) = 2^n - 1$ as the divisors of $2^{n - 1}$ are all powers of $2$ up to
  and including $2^{n - 1}$:

  \begin{align*}
    1 + 2 + 4 + 8 + ... + 2^{n - 1} \\
    = 2^0 + 2^1 + 2^2 + 2^3 + ... + 2^{n - 1}
  \end{align*}

  \noindent
  The above is just a geometric series, whose sum can be computed using the formula 
  $S_{n} = \frac{1 - r^{n + 1}}{1 - r}$ (source: \href{https://mathworld.wolfram.com/GeometricSeries.html}{https://mathworld.wolfram.com/GeometricSeries.html}) 
  where $r$ is the common ratio, and $n$ is the number of terms.
  \spacing

  \noindent
  In this case, $r = 2$ and $n = n - 1$. This gives us enough information to compute the sum:

  \begin{align*}
    S_{n} &= \frac{1 - 2^{(n - 1) + 1}}{1 - 2} \\
      &= \frac{1 - 2^n}{-1} \\
      &= 2^n - 1
  \end{align*}

  \spacing

  \noindent
  Lastly, we must notice that our function $\sigma(n)$ is multiplicative, that is $\sigma(ab) = \sigma(a) \cdot \sigma(b)$, 
  if $a$ and $b$ are relatively prime. I won't prove this here, but link to a wikipedia article that explains more
  about the function and its properties: \href{https://en.wikipedia.org/wiki/Divisor_function}{https://en.wikipedia.org/wiki/Divisor\_function}.
  \spacing

  \noindent
  For the purposes of this proof, we know that $2^n - 1$ and $2^{n - 1}$ are relatively prime, so our function $\sigma(n)$
  is multiplicative for the numbers $2^n - 1$ and $2^{n - 1}$.
  \spacing

  \noindent
  Putting it all together:

  \begin{align*}
    \sigma(2^{n - 1}(2^{n} - 1)) &= \sigma(2^{n - 1})\sigma(2^n - 1) && \text{[Multiplicative property]} \\
      &= (2^n - 1)(2^n) && \text{[Replace with sums]} \\
      &= 2(2^{n - 1})(2^n - 1) && \text{[Factor out a 2]}
  \end{align*}

  \noindent
  Therefore $2^n-1(2^n - 1)$ is a perfect number as $\frac{\sigma(2^{n - 1}(2^{n} - 1))}{2} = 2^{n - 1}(2^{n} - 1)$.
\end{proof}

\newpage
\subsection*{Problem 2}

\underline{Step 1:} Find $148^{-1}$ (mod 421)
\spacing

\noindent
Compute the steps of the Euclidean $GCD$ algorithm:

\begin{align*}
  421 &= 2 \times 148 + 125 \\
  148 &= 1 \times 125 + 23 \\
  125 &= 5 \times 23 + 10 \\
  23 &= 2 \times 10 + 3 \\
  10 &= 3 \times 3 + 1
\end{align*}

\spacing
\noindent
Roll back the steps to find $s, t \in \Z$ such that $1 = 421s + 148t$

\begin{align*}
  1 &= 1(10) - 3(3) \\
    &= 1(10) - 3(23 - 2(10)) \\
    &= 7(10) - 3(23) \\
    &= 7(125 - 5(23)) - 3(23) \\
    &= 7(125) - 38(23) \\
    &= 7(125) - 38(148 - 1(125)) \\
    &= 45(125) - 38(148) \\
    &= 45(421 - 2(148)) - 38(148) \\
    &= 45(421) - 128(148)
\end{align*}

\spacing
\noindent
So $1 = 45(421) - 128(148)$, we then get $1 = -128(148)$, 
hence $148^{-1}$ (mod 421) $\equiv -128 \equiv 293$ (mod 421).
\spacing

\noindent
\underline{Step 2}: Solve $148x \equiv 12$ (mod 421)

\begin{align*}
  148x &\equiv 12 \text{ (mod 421)} \\
     x &\equiv 12 \times 293 \text{ (mod 421)} \\
       &\equiv 3516 \text{ (mod 421)} \\
       &\equiv 148 \text{ (mod 421)}
\end{align*}

\newpage
\subsection*{Problem 3}

Recall: $a^{p - 1} \equiv 1 \text{ (mod p)}$

\subsubsection*{(a)}

First we try to decompose $1335$ into $(18 \cdot n) + r$.
\spacing

\intlongdivision{1335}{18}
\spacing

\noindent
Therefore $n = 74$ and $r = 3$

\begin{align*}
  2409^{1335} \text{ (mod 19)} &= 2409^{(18 \cdot 74) + 3} \text{ (mod 19)} \\
    &= 2409^3 \text{ (mod 19)} && \text{[$2409 \equiv 15$ (mod 19) by LD]} \\
    &= 15^3 \text{ (mod 19)} \\
    &= 3375 \text{ (mod 19)} && \text{[Perform LD on (3375, 19)]} \\
    &= 12 \text{ (mod 19)}
\end{align*}

\subsubsection*{(b)}

First we try to decompose $42806$ into $(348 \cdot n) + r$.
\spacing

\intlongdivision{42806}{348}
\spacing

\noindent
Therefore $n = 123$ and $r = 2$.

\begin{align*}
  7^{42806} \text{ (mod 349)} &= 7^{(123 \cdot 348) + 2} \text{ (mod 349)} \\
    &= 7^2 \text{ (mod 349)} \\
    &= 49 \text{ (mod 349)}
\end{align*}

\newpage
\subsection*{Problem 4}

\subsubsection*{(a)}

\begin{align*}
  \hat{M} &= M^p \text{ mod n} \\
    &= 4^5 \text{ mod 91} \\
    &= 1024 \text{ mod 91} \\
    &= 23
\end{align*}

\subsubsection*{(b)}

\begin{align*}
  x &= p^{-1} \text{ mod $(q_{1} - 1)(q_{2} - 1)$} \\
    &= 5^{-1} \text{ mod 72}
\end{align*}

\spacing
\noindent
Compute the steps of the Euclidean $GCD$ algorithm:

\begin{align*}
  72 &= 14 \times 5 + 2 \\
  5 &= 2 \times 2 + 1
\end{align*}

\spacing
\noindent
Roll back the steps to find $s, t \in \Z$ such that $1 = 5s + 72t$

\begin{align*}
  1 &= 5 - 2(2) \\
    &= 5 - 2(72 - 14(5)) \\
    &= 29(5) - 2(72)
\end{align*}

\noindent
So we see that $x = 29$, since $p \cdot 29 \equiv 1$ mod $72$.

\subsubsection*{(c)}

\begin{align*}
  M &= \hat{M}^x \text{ mod n} \\
    &= 23^{29} \text{ mod 91} \\
\end{align*}

\noindent
We know that $91 = 7 \cdot 13$, therefore by the Chinese Remainder Theorem a solution to
$23^{29} \text{ mod 7}$ is also a solution to our original equation:

\begin{align*}
  M &= \hat{M}^x \text{ mod n} \\
    &= 23^{29} \text{ mod 91} \\
    &= 23^{29} \text{ mod 7} \\
    &= 23^{(7 \cdot 3) + 2} \text{ mod 7} \\
    &= 23^2 \text{ mod 7} \\
    &= 529 \text{ mod 7}
\end{align*}

\noindent
Perform long division on the integers $529$ and $7$:

\intlongdivision{529}{7}
\spacing

\noindent
Therefore our answer is $4$.

\end{document}